metrics/LipExt.v
@@ -1,0 +1,414 @@
+(*  
+
+Formalization of the theorem about extension of real-valued Lipschitz
+functions. This theorem originally belongs to McShane and Kirchbraun. 
+
+Theorem. Let M - metric space, let X - subset of M. Let f - Lipschitz
+function from X to reals with constant C. Then the function defined by 
+
+\tilde f (y) = inf_{x \in X} { f(x) + C * d_M (x, y)}
+
+is the extension of f and has the same Lipshitz constant.
+
+The constructive proof also has a restriction on totally boundness of
+subset X.
+
+*)
+
+Require Import ContFunctions.
+Require Import CMetricSpaces.
+Require Import CPMSTheory.
+
+Variable M : CMetricSpace.
+Variable P : M -> CProp.
+Variable C : IR.
+Variable f : CSetoid_fun (SubMetricSpace M P) IR_as_CMetricSpace.
+
+Hypothesis set_bounded : MStotally_bounded (SubMetricSpace M P).
+Hypothesis non_empty : {x : M | P x}.
+Hypothesis constant_positive : Zero[<]C.
+
+Hypothesis f_lip : lipschitz_c f C.
+
+Section BuildExtension.
+
+Definition cdsub' (y : M) : CSetoid_fun (SubMetricSpace M P) IR_as_CMetricSpace.
+intros.
+apply Build_CSetoid_fun with (fun x : (SubMetricSpace M P) => 
+C [*] (dsub' M P y x)).
+red. intros x y0 H1.
+elim (bin_op_strext_unfolded _ _ _ _ _ _ H1).
+intros H3.
+elim (ap_irreflexive_unfolded _ _ H3).
+intros H3.
+apply (dsub'_strext M P y); auto.
+Defined.
+
+Lemma f_uni_cont: uni_continuous f.
+assert (lipschitz' f).
+apply (lip_c_imp_lip (SubMetricSpace M P) IR_as_CMetricSpace f C).
+apply f_lip.
+assert (lipschitz f).
+apply (lipschitz'_imp_lipschitz (SubMetricSpace M P) IR_as_CMetricSpace f); auto.
+apply lipschitz_imp_uni_continuous; auto.
+Qed.
+
+Lemma dsub'_is_lipschitz :
+forall (y : M) (x1 x2 : SubMetricSpace M P),
+C[*]dIR (dsub' M P y x1) (dsub' M P y x2)[<=]C[*](dsub M P x1 x2).
+intros.
+apply mult_resp_leEq_lft.
+2: apply less_leEq.
+2: apply constant_positive.
+unfold dsub'. unfold dsub.
+case x1. case x2. intros. simpl.
+
+astepl (dIR (y[-d]scs_elem0) (y[-d]scs_elem)).
+apply rev_tri_ineq'.
+
+unfold dIR.
+apply ABSIR_wd.
+assert ((y[-d]scs_elem0)[=](scs_elem0[-d]y)).
+apply ax_d_com.
+apply CPsMetricSpace_is_CPsMetricSpace.
+assert ((y[-d]scs_elem)[=](scs_elem[-d]y)).
+apply ax_d_com.
+apply CPsMetricSpace_is_CPsMetricSpace.
+Algebra.
+Qed.
+
+
+Lemma exp_prop : forall (k : nat) (n : nat) (H : Two[#]Zero),
+Two[^]k[*]nexp IR (n + k) (One[/] (Two:IR)[//]H)[=]
+nexp IR n (One[/] (Two:IR)[//]H).
+intros.
+astepl ((zexp Two H k)[*](nexp IR (n + k) (One[/] Two[//]H) )).
+astepl ((zexp Two H k)[*](zexp Two H (- (n + k)%nat))).
+astepr (zexp Two H (k + (- (n + k)%nat))).
+apply eq_symmetric.
+apply zexp_plus.
+astepl (zexp Two H (-n)).
+apply (zexp_inv_nexp IR Two H n).
+replace (- n)%Z with (k + - (n + k)%nat)%Z; auto with zarith.
+apply eq_reflexive.
+intros. auto with zarith.
+assert ((n + k)%Z = (n + k)%nat). 
+symmetry. apply inj_plus.
+auto with zarith.
+apply mult_wd; auto.
+apply eq_reflexive.
+apply (zexp_inv_nexp IR Two H (n+k)).
+Qed.
+
+Lemma cdsub'_uni_cont : forall y : M, uni_continuous (cdsub' y).
+intros.
+unfold uni_continuous.
+unfold cdsub'.
+simpl.
+intros.
+elim (power_big C Two). intros k H1.
+3: apply one_less_two.
+2: apply less_leEq; apply constant_positive.
+exists (n + k).
+intros.
+astepl (C[*](dIR (dsub' M P y x) (dsub' M P y y0))).
+cut (C[*]dIR (dsub' M P y x) (dsub' M P y y0)[<=]C[*](dsub M P x y0)).
+intros.
+cut (C[*](dsub M P x y0)[<] nexp IR n (One[/] Two[//]H)).
+intros.
+apply leEq_less_trans with (C[*](dsub M P x y0)); auto with algebra.
+cut (Two[^]k[*](dsub M P x y0)[<] nexp IR n (One[/] Two[//]H)).
+intros.
+cut (C[*](dsub M P x y0)[<=]Two[^]k[*](dsub M P x y0)).
+intros.
+apply leEq_less_trans with (Two[^]k[*](dsub M P x y0)); auto with algebra.
+apply mult_resp_leEq_rht; auto.
+apply dsub_nneg.
+astepr (Two[^]k[*](nexp IR (n + k) (One[/] Two[//]H))).
+apply mult_resp_less_lft; auto.
+apply nexp_resp_pos.
+cut ((One:IR)[<]Two).
+cut (Zero[<](One:IR)).
+intros.
+apply less_transitive_unfolded with (One:IR); auto.
+apply pos_one.
+apply one_less_two.
+apply exp_prop.
+apply dsub'_is_lipschitz.
+unfold dIR.
+astepr (ABSIR (C[*](dsub' M P y x[-]dsub' M P y y0))).
+apply AbsIR_mult.
+apply constant_positive.
+apply ABSIR_wd; auto with algebra.
+Qed.
+
+Definition f_multi_ext (y : M) : CSetoid_fun (SubMetricSpace M P) IR_as_CMetricSpace.
+intros.
+apply Build_CSetoid_fun with (fun x : (SubMetricSpace M P) => 
+f (x) [+] (cdsub' y x)).
+red. intros x y0 H1.
+elim (bin_op_strext_unfolded _ _ _ _ _ _ H1).
+apply (csf_strext (SubMetricSpace M P) IR_as_CMetricSpace f).
+apply (csf_strext (SubMetricSpace M P) IR_as_CMetricSpace (cdsub' y)).
+Defined.
+
+Lemma f_multi_ext_uni_continuous :  forall y : M, uni_continuous (A:=SubMetricSpace M P) (B:=IR_as_CPsMetricSpace)
+     (f_multi_ext y).
+intros.
+unfold f_multi_ext.
+apply (plus_resp_uni_continuous (SubMetricSpace M P) f (cdsub' y)
+	f_uni_cont (cdsub'_uni_cont y)).
+Qed.
+
+Lemma inf_f_multi_ext_exists :
+forall y : M, {z : IR | set_glb_IR (fun v : IR_as_CMetricSpace => {x : SubMetricSpace M P | f_multi_ext y x[=]v}) z}.
+intros.
+elim (infimum_exists (SubMetricSpace M P) (f_multi_ext y)).
+3: apply set_bounded.
+intros x H.
+exists x.
+apply H.
+assert (uni_continuous (f_multi_ext y)).
+apply f_multi_ext_uni_continuous.
+assert (uni_continuous' (f_multi_ext y)).
+apply uni_continuous_imp_uni_continuous'; auto.
+apply uni_continuous'_imp_uni_continuous''; auto.
+elim non_empty.
+intros x H.
+exists x. apply H.
+Qed.
+
+Definition lip_extension_f (y : M) : IR.
+intros.
+assert ({z : IR | set_glb_IR (fun v : IR_as_CMetricSpace => {x : SubMetricSpace M P | f_multi_ext y x[=]v}) z}).
+apply inf_f_multi_ext_exists.
+destruct X.
+exact x.
+Defined. 
+
+Lemma lip_extension_strext_case: forall (x : M) (y : M)
+  (z1 : IR)  (z2 : IR)  (H : z1[<]z2)
+  (H1 : set_glb_IR
+         (fun v : IR =>
+          sigT (fun x : subcsetoid_crr M P => f x[+]C[*]dsub' M P y x[=]v))
+         z1)
+  (H2 : set_glb_IR
+         (fun v : IR =>
+          sigT (fun x0 : subcsetoid_crr M P => f x0[+]C[*]dsub' M P x x0[=]v))
+         z2), x [#] y.
+unfold set_glb_IR.
+intros.
+destruct H1. destruct H2.
+assert {x0 : IR |
+    sigT (fun x1 : subcsetoid_crr M P => f x1[+]C[*]dsub' M P y x1[=]x0) |
+    x0[-]z1[<](z2 [-] z1)}.
+apply s.
+apply shift_zero_less_minus; auto.
+destruct X. destruct s1.
+assert (z2[<=]f x1[+]C[*]dsub' M P x x1).
+apply (l0 (f x1[+]C[*]dsub' M P x x1)).
+exists x1.
+Algebra.
+assert (x0 [<] z2).
+apply plus_cancel_less with ([--]z1). Algebra.
+assert (f x1[+]C[*]dsub' M P y x1 [<] f x1[+]C[*]dsub' M P x x1).
+apply less_leEq_trans with z2; auto.
+astepl (x0). auto.
+assert ((from_SubPsMetricSpace M P x1[-d] y)[#](from_SubPsMetricSpace M P x1[-d]x)).
+apply less_imp_ap.
+apply mult_cancel_less with (z := C).
+apply constant_positive.
+astepl (C[*]dsub' M P y x1).
+astepr (C[*]dsub' M P x x1).
+apply plus_cancel_less with (f x1).
+astepl (f x1[+]C[*]dsub' M P y x1).
+astepr (f x1[+]C[*]dsub' M P x x1).
+auto.
+set (H1 := csbf_strext _ _ _ (cms_d (c:=M)) _ _ _ _ X1).
+elim H1.
+assert (Not (from_SubPsMetricSpace M P x1[#]from_SubPsMetricSpace M P x1)).
+apply ap_irreflexive_unfolded.
+contradiction.
+intros.
+apply ap_symmetric_unfolded.
+auto.
+Qed.
+
+Lemma lip_extension_strext :
+ fun_strext (lip_extension_f).
+unfold fun_strext.
+unfold lip_extension_f.
+intros x y.
+elim inf_f_multi_ext_exists.
+elim inf_f_multi_ext_exists.
+simpl. intros z1 H1 z2 H2 H.
+elim (ap_imp_less IR z1 z2); auto; intros.
+unfold f_multi_ext.
+apply (lip_extension_strext_case x y z1 z2 a H1 H2).
+apply ap_symmetric_unfolded.
+apply (lip_extension_strext_case y x z2 z1 b H2 H1).
+apply ap_symmetric_unfolded. auto.
+Qed.
+
+Definition lip_extension :=
+  Build_CSetoid_fun M IR_as_CPsMetricSpace (lip_extension_f)
+   (lip_extension_strext).
+   
+Lemma lip_unfolded : forall (x x1: SubMetricSpace M P),
+f x[-]f x1[<=]C[*]dsub' M P (from_SubPsMetricSpace M P x) x1.
+intros.
+unfold dsub'.
+astepr (C[*](x[-d]x1)).
+apply leEq_transitive with (AbsIR (f x[-] f x1)).
+apply leEq_AbsIR.
+astepl (f x[-d]f x1).
+assert (lipschitz_c f C).
+apply f_lip.
+apply X.
+apply mult_wd; Algebra.
+case x. case x1. intros. simpl.
+apply ax_d_com.
+apply CPsMetricSpace_is_CPsMetricSpace.
+Qed.
+
+
+End BuildExtension.
+
+Section ExtensionProperties.
+
+Lemma lip_extension_keeps_fun : forall (x : SubMetricSpace M P),
+lip_extension (from_SubPsMetricSpace M P x) [=] f x.
+intros.
+unfold lip_extension. 
+simpl.
+unfold lip_extension_f.
+elim inf_f_multi_ext_exists.
+unfold set_glb_IR.
+simpl. intros y H.
+destruct H.
+
+apply leEq_imp_eq.
+
+apply l.
+exists x.
+assert (dsub' M P (from_SubPsMetricSpace M P x) x[=]Zero).
+unfold dsub'.
+
+assert (diag_zero M (cms_d (c:=M))).
+apply pos_imp_ap_imp_diag_zero.
+apply ax_d_pos_imp_ap.
+apply (CPsMetricSpace_is_CPsMetricSpace M). 
+apply ax_d_nneg.
+apply (CPsMetricSpace_is_CPsMetricSpace M). 
+apply H.
+
+astepl (f x[+]C[*]Zero).
+astepl (f x[+]Zero). Algebra.
+
+assert (forall e : IR, Zero [<]e -> f x [-] y [<] e).
+intros.
+assert (sig2T IR
+        (fun x0 : IR =>
+         sigT
+            (fun x1 : subcsetoid_crr M P =>
+        f x1[+]C[*]dsub' M P (from_SubPsMetricSpace M P x) x1[=]x0))
+        (fun x : IR => x[-]y[<]e)).
+apply s. auto. destruct X0. destruct s0.
+assert (f x [<=] f x1[+]C[*]dsub' M P (from_SubPsMetricSpace M P x) x1).
+astepr (C[*] dsub' M P (from_SubPsMetricSpace M P x) x1 [+] f x1).
+apply shift_leEq_plus.
+apply lip_unfolded.
+apply leEq_less_trans with (f x1[+]C[*]dsub' M P (from_SubPsMetricSpace M P x) x1[-]y).
+apply minus_resp_leEq; auto.
+astepl (x0 [-] y); auto.
+astepl (f x [-] y [+] y).
+astepr (Zero [+] y).
+apply plus_resp_leEq.
+unfold leEq.
+apply approach_zero; auto.
+Qed.
+
+Lemma extension_also_lipschitz_case :
+forall (y1 : M) (y2 : M) (fy2 : IR) 
+(Hfy2 : set_glb_IR (fun v : IR =>
+  sigT (fun x : subcsetoid_crr M P => f x[+]C[*]dsub' M P y2 x[=]v)) fy2)
+(fy1 : IR)
+(Hfy1 : set_glb_IR (fun v : IR =>
+ sigT (fun x : subcsetoid_crr M P => f x[+]C[*]dsub' M P y1 x[=]v))  fy1)
+(e : IR)
+(X : Zero[<]e),
+fy2[-]fy1[<=]C[*](y1[-d]y2)[+]e.
+intros.
+destruct Hfy1. destruct Hfy2.
+assert ({x : IR | sigT (fun x0 : SubMetricSpace M P => f x0[+]C[*]dsub' M P y1 x0[=]x) |
+      x[-]fy1[<]e}).
+apply s. auto. destruct X0 as [fx1 Ht Hl1].  destruct Ht as [x1 He1].
+
+assert (fy2 [<=] f x1[+]C[*]dsub' M P y2 x1).
+apply l0; auto. exists x1. apply eq_reflexive_unfolded.
+
+assert (fx1[-]e[<=]fy1).
+apply less_leEq.
+apply shift_minus_less.
+apply shift_less_plus'; auto.
+
+(* Inequalites are simple and symmetric*)
+
+apply leEq_transitive with ((f x1[+]C[*]dsub' M P y2 x1)[-](fx1[-]e)).
+apply minus_resp_leEq_both; auto.
+astepl (f x1[+]C[*]dsub' M P y2 x1[-]fx1[+]e).
+apply plus_resp_leEq.
+astepl (f x1[+]C[*]dsub' M P y2 x1[-](f x1[+]C[*]dsub' M P y1 x1)).
+astepl (f x1[+]C[*]dsub' M P y2 x1[-]f x1[-]C[*]dsub' M P y1 x1).
+astepl (f x1[-]f x1[+]C[*]dsub' M P y2 x1[-]C[*]dsub' M P y1 x1).
+astepl (Zero[+]C[*]dsub' M P y2 x1[-]C[*]dsub' M P y1 x1).
+astepl (C[*]dsub' M P y2 x1[-]C[*]dsub' M P y1 x1).
+astepl (C[*](dsub' M P y2 x1[-]dsub' M P y1 x1)).
+apply mult_resp_leEq_lft.
+2: apply less_leEq.
+2: apply constant_positive.
+unfold dsub'.
+astepr (y2[-d]y1).
+apply leEq_transitive with (AbsIR ((from_SubPsMetricSpace M P x1[-d]y2)[-]
+			    (from_SubPsMetricSpace M P x1[-d]y1))).
+apply leEq_AbsIR.
+apply AbsSmall_imp_AbsIR.
+apply rev_tri_ineq.
+apply ax_d_com.
+apply CPsMetricSpace_is_CPsMetricSpace.
+rational.
+Qed.
+
+Lemma extension_also_liscphitz : lipschitz_c (lip_extension) C.
+unfold lipschitz_c.
+unfold lip_extension.
+unfold lip_extension_f.
+intros y1 y2. intros. simpl.
+elim inf_f_multi_ext_exists.
+elim inf_f_multi_ext_exists.
+unfold f_multi_ext.
+unfold dIR.
+simpl.
+intros fy2 Hfy2 fy1 Hfy1.
+apply AbsSmall_imp_AbsIR.
+
+assert (forall e : IR, Zero[<]e -> AbsSmall (C[*](y1[-d]y2)[+]e) (fy1[-]fy2)).
+
+intros.
+unfold AbsSmall. split.
+astepr ([--](fy2 [-] fy1)).
+apply inv_resp_leEq.
+apply extension_also_lipschitz_case; auto.
+rational.
+astepr (C[*](y2[-d]y1)[+]e).
+astepl (fy1 [-] fy2).
+apply (extension_also_lipschitz_case y2 y1 fy1 Hfy1 fy2 Hfy2 e X).
+assert (y2[-d]y1[=]y1[-d]y2).
+apply ax_d_com.
+apply CPsMetricSpace_is_CPsMetricSpace.
+Algebra.
+apply AbsSmall_approach. auto.
+Qed.
+
+End ExtensionProperties.
+
